theories/hlogic.v
@@ -1,0 +1,810 @@
+From stdpp Require Export gmap.
+From iris.bi Require Export interface.
+From iris.algebra Require Import excl gmap auth.
+From iris.proofmode Require Export tactics.
+Require Export diris.langdef.
+Require Export diris.logic.bi.
+Require Export diris.util.
+Require Export diris.logic.bupd.
+Ltac inv H := inversion H; clear H; simpl in *; simplify_eq.
+
+Lemma other_neq ep :
+  ep ≠ other ep.
+Proof.
+  by destruct ep,b.
+Qed.
+
+Inductive owner :=
+  | Thread : nat -> owner
+  | Chan : chan -> owner.
+
+Instance owner_eqdecision : EqDecision owner.
+Proof.
+  intros [n|n] [m|m]; unfold Decision; destruct (decide (n = m));
+  subst; eauto; right; intro; simplify_eq.
+Qed.
+Instance owner_countable : Countable owner.
+Proof.
+  refine (inj_countable' (λ l, match l with
+  | Thread n => inl n
+  | Chan n => inr n
+  end) (λ l, match l with
+  | inl n => Thread n
+  | inr n => Chan n
+  end) _); by intros [].
+Qed.
+
+Canonical Structure ownerO := leibnizO owner.
+Canonical Structure chan_typeO := leibnizO chan_type.
+
+Notation heapT := (gmap endpoint chan_type).
+Notation heapTO := (gmap endpoint (chan_type * owner)).
+Notation heapT_UR := (gmapUR endpoint (exclR chan_typeO)).
+Notation heapTO_UR := (gmapUR endpoint (exclR (prodO chan_typeO ownerO))).
+
+Notation oProp := (uPred heapT_UR).
+Notation iProp := (uPred (authUR heapTO_UR)).
+
+Notation "⌜⌜ p ⌝⌝" := (<affine> ⌜ p ⌝)%I : bi_scope.
+
+Definition attach_owner (o : owner) (h : heapT) : heapTO := (λ t, (t,o)) <$> h.
+
+Section attach_owner.
+  Lemma attach_owner_empty o : attach_owner o ∅ = ∅.
+  Proof. rewrite /attach_owner fmap_empty //. Qed.
+  Lemma attach_owner_union o m1 m2 :
+    attach_owner o (m1 ∪ m2) = attach_owner o m1 ∪ attach_owner o m2.
+  Proof. rewrite /attach_owner map_fmap_union //. Qed.
+  Lemma fmap_map_disjoint `{Countable K} {V1 V2} (f : V1 -> V2) (m1 m2 : gmap K V1) :
+    m1 ##ₘ m2 <-> f <$> m1 ##ₘ f <$> m2.
+  Proof.
+    split.
+    - intros HH.
+      intros x. rewrite !lookup_fmap.
+      specialize (HH x).
+      destruct (m1 !! x); destruct (m2 !! x); try done.
+    - intros HH.
+      intros x. specialize (HH x).
+      rewrite !lookup_fmap in HH.
+      destruct (m1 !! x); destruct (m2 !! x); try done.
+  Qed.
+  Lemma attach_owner_disj o m1 m2 :
+    m1 ##ₘ m2 <-> attach_owner o m1 ##ₘ attach_owner o m2.
+  Proof. apply fmap_map_disjoint. Qed.
+End attach_owner.
+
+Definition map_Excl `{Countable K} {V} (m : gmap K V) : gmap K (excl V) := Excl <$> m.
+
+Section map_Excl.
+  Context `{Countable K} {V : ofeT} `{!LeibnizEquiv V}.
+  Implicit Type m : gmap K V.
+  Lemma map_Excl_valid m : ✓ (map_Excl m).
+  Proof. intros i. rewrite /map_Excl lookup_fmap. destruct (m !! i); done. Qed.
+  Lemma map_Excl_empty : map_Excl ∅ = (ε : gmap K (excl V)).
+  Proof. rewrite /map_Excl fmap_empty. done. Qed.
+  Lemma map_Excl_insert m k v :
+    map_Excl (<[ k := v ]> m) = <[ k := Excl v ]> $ map_Excl m.
+  Proof.
+    rewrite /map_Excl fmap_insert //.
+  Qed.
+  Lemma map_Excl_insert_op m k v :
+    m !! k = None ->
+    map_Excl (<[ k := v ]> m) = {[ k := Excl v ]} ⋅ map_Excl m.
+  Proof.
+    intros HH.
+    rewrite /map_Excl fmap_insert insert_singleton_op //
+            lookup_fmap HH //.
+  Qed.
+  Lemma map_Excl_union m1 m2 :
+    m1 ##ₘ m2 -> map_Excl (m1 ∪ m2) = map_Excl m1 ⋅ map_Excl m2.
+  Proof.
+    induction m1 using map_ind; intros; decompose_map_disjoint.
+    - by rewrite map_Excl_empty !left_id_L.
+    - assert ((m ∪ m2) !! i = None).
+      { rewrite lookup_union H0 H1 //. }
+      rewrite -insert_union_l !map_Excl_insert_op // IHm1 // assoc_L //.
+  Qed.
+  Lemma map_Excl_singleton_op_inv m me k x :
+    map_Excl m = {[ k := Excl x ]} ⋅ me ->
+    ∃ m', m = <[ k := x ]> m' ∧ me = map_Excl m' ∧ m' !! k = None.
+  Proof.
+    rewrite /map_Excl. intros HH.
+    exists (delete k m).
+    assert (m !! k = Some x).
+    { rewrite ->map_eq_iff in HH.
+      specialize (HH k).
+      revert HH. rewrite lookup_fmap lookup_op lookup_singleton.
+      case: (m!!k); case:(me!!k); simpl; intros; inversion HH. done. }
+    rewrite !map_eq_iff.
+    rewrite-> map_eq_iff in HH.
+    split_and!.
+    - intros i.
+      destruct (decide (k = i)); subst.
+      + rewrite lookup_insert //.
+      + rewrite lookup_insert_ne // lookup_delete_ne //.
+    - intros i.
+      specialize (HH i).
+      destruct (decide (k = i)); subst.
+      + rewrite lookup_fmap lookup_delete.
+        revert HH. rewrite !lookup_fmap lookup_op lookup_singleton H0 /=.
+        case: (me !! i); eauto.
+        intros a HH. inversion HH.
+      + rewrite lookup_fmap lookup_delete_ne //.
+        revert HH. rewrite lookup_fmap lookup_op lookup_singleton_ne //.
+        case: (me !! i); simpl; intros; rewrite HH //.
+    - rewrite lookup_delete //.
+  Qed.
+  Lemma map_Excl_union_inv m me1 me2 :
+    map_Excl m = me1 ⋅ me2 ->
+    ∃ m1 m2, m = m1 ∪ m2 ∧ me1 = map_Excl m1 ∧ me2 = map_Excl m2 ∧ m1 ##ₘ m2.
+  Proof.
+    revert m. induction me1 as [|k xe me1 Hx IH] using map_ind; intros m.
+    - rewrite left_id_L. intros <-.
+      exists ∅,m.
+      rewrite left_id_L map_Excl_empty. split_and!; solve_map_disjoint.
+    - rewrite insert_singleton_op // -assoc_L.
+      destruct xe as [x|].
+      + intros (m' & -> & ? & ?)%map_Excl_singleton_op_inv.
+        destruct (IH m') as (m1 & m2 & -> & -> & -> & ?); first done.
+        exists (<[ k := x]> m1),m2.
+        apply lookup_union_None in H1 as [].
+        repeat split.
+        * by rewrite insert_union_l.
+        * rewrite map_Excl_insert_op //.
+        * by apply map_disjoint_insert_l.
+      + intros Hm. assert (✓ (ExclBot : excl V)) as [].
+        eapply (singleton_valid k), (cmra_valid_op_l _ (me1 ⋅ me2)).
+        rewrite -Hm. apply map_Excl_valid.
+  Qed.
+  Lemma map_Excl_disjoint m1 m2 :
+    m1 ##ₘ m2 <-> map_Excl m1 ##ₘ map_Excl m2.
+  Proof. apply fmap_map_disjoint. Qed.
+End map_Excl.
+
+Definition owned (o : owner) (P : oProp) : iProp :=
+  ∃ (h : heapT),
+    ⌜⌜ uPred_holds P (map_Excl h) ⌝⌝ ∗
+    uPred_ownM (◯ (map_Excl $ attach_owner o h)).
+
+Lemma owned_mono (P Q : oProp) o :
+  (P ⊢ Q) → owned o P ⊢ owned o Q.
+Proof.
+  iIntros (H) "H". unfold owned.
+  iDestruct "H" as (h H1) "H".
+  iExists h. iFrame. iPureIntro.
+  apply H; last done.
+  intros i. rewrite lookup_fmap. case: (h !! i); done.
+Qed.
+
+Instance owned_proper_vdash o : Proper ((⊢) ==> (⊢)) (owned o).
+Proof. intros ???. by apply owned_mono. Qed.
+Instance owned_proper_flip_vdash o : Proper (flip (⊢) ==> flip (⊢)) (owned o).
+Proof. intros ???. simpl in *. by apply owned_mono. Qed.
+Instance: Params (owned) 1 := {}.
+Instance owned_proper_equiv o : Proper ((≡) ==> (≡)) (owned o).
+Proof.
+  intros P1 P2 [HP1 HP2]%bi.equiv_spec; apply bi.equiv_spec. split.
+    - by rewrite HP1.
+    - by rewrite HP2.
+Qed.
+
+(*
+Talk to Robbert about these Coq issues,
+and being stuck on stupid stuff => frustration => low motivation
+*)
+Section uPred_lemmas.
+  Context {A : ucmraT}.
+  Implicit Types P Q : uPred A.
+  Arguments uPred_holds {_} !_/.
+  Lemma owned_emp_helper (x : A) : ✓ x -> (uPred_ownM x ⊢ emp) -> x ≡ ε.
+  Proof.
+    uPred.unseal. intros ? [H]. apply H; simpl; done.
+  Qed.
+
+  Lemma uPred_emp_holds x :
+    (emp%I : uPred A) x <-> x ≡ ε.
+  Proof. by uPred.unseal. Qed.
+  Lemma uPred_emp_holds_L `{!LeibnizEquiv A} x :
+    (emp%I : uPred A) x <-> x = ε.
+  Proof. unfold_leibniz. apply uPred_emp_holds. Qed.
+
+  Lemma uPred_sep_holds P Q x :
+    (P ∗ Q)%I x <-> ∃ x1 x2, x ≡ x1 ⋅ x2 ∧ P x1 ∧ Q x2.
+  Proof. by uPred.unseal. Qed.
+  Lemma uPred_sep_holds_L `{!LeibnizEquiv A} P Q x :
+    (P ∗ Q)%I x <-> ∃ x1 x2, x = x1 ⋅ x2 ∧ P x1 ∧ Q x2.
+  Proof. unfold_leibniz. apply uPred_sep_holds. Qed.
+
+  Lemma uPred_and_holds P Q x :
+    (P ∧ Q)%I x <-> P x ∧ Q x.
+  Proof. by uPred.unseal. Qed.
+  Lemma uPred_pure_holds φ x :
+    (⌜ φ ⌝ : uPred A)%I x <-> φ.
+  Proof. by uPred.unseal. Qed.
+  Lemma uPred_exists_holds {B} (Φ : B -> uPred A) x :
+    (∃ b, Φ b)%I x <-> ∃ b, Φ b x.
+  Proof. by uPred.unseal. Qed.
+  Lemma uPred_affinely_pure_holds φ x :
+    (⌜⌜ φ ⌝⌝ : uPred A)%I x <-> x ≡ ε ∧ φ.
+  Proof. rewrite /bi_affinely uPred_and_holds uPred_pure_holds uPred_emp_holds. done. Qed.
+  Lemma uPred_affinely_pure_holds_L `{!LeibnizEquiv A} φ x :
+    (⌜⌜ φ ⌝⌝ : uPred A)%I x <-> x = ε ∧ φ.
+  Proof. unfold_leibniz. apply uPred_affinely_pure_holds. Qed.
+End uPred_lemmas.
+
+Lemma owned_pure φ o :
+  owned o ⌜⌜ φ ⌝⌝ ⊣⊢ ⌜⌜ φ ⌝⌝.
+Proof.
+  rewrite /owned.
+  setoid_rewrite uPred_affinely_pure_holds_L.
+  iSplit.
+  - iIntros "H". iDestruct "H" as (h []) "H".
+    apply (fmap_empty_inv Excl h) in H as ->.
+    rewrite attach_owner_empty map_Excl_empty uPred.ownM_unit //.
+  - iIntros (H). iExists ∅.
+    iSplit.
+    + iPureIntro. rewrite map_Excl_empty //.
+    + rewrite attach_owner_empty map_Excl_empty uPred.ownM_unit //.
+Qed.
+
+Lemma owned_emp o :
+  owned o emp ⊣⊢ emp.
+Proof.
+  Search emp%I (<affine> emp)%I.
+  rewrite -bi.affinely_emp.
+  rewrite -bi.affinely_True_emp.
+  rewrite owned_pure.
+  rewrite bi.affinely_True_emp.
+  rewrite bi.affinely_emp.
+  done.
+Qed.
+
+Lemma uPred_ownM_disjoint (m1 m2 : heapTO) :
+  uPred_ownM (◯ (map_Excl m1)) -∗ uPred_ownM (◯ (map_Excl m2)) -∗ ⌜ m1 ##ₘ m2 ⌝.
+Proof.
+  iIntros "H1 H2".
+  iDestruct (uPred.ownM_op with "[H1 H2]") as "H"; first iFrame.
+  rewrite -auth_frag_op.
+  rewrite uPred_primitive.ownM_valid.
+  rewrite auth_frag_valid.
+  iDestruct "H" as "%". iPureIntro.
+  apply map_Excl_disjoint.
+  intros x. specialize (H x).
+  rewrite lookup_op in H.
+  destruct (_ !! x);
+  destruct (_ !! x); done.
+Qed.
+
+Lemma owned_sep (P Q : oProp) o :
+  owned o (P ∗ Q) ⊣⊢ owned o P ∗ owned o Q.
+Proof.
+  unfold owned.
+  setoid_rewrite uPred_sep_holds_L.
+  iSplit; iIntros "H".
+  - iDestruct "H" as (h H) "H".
+    destruct H as (x1 & x2 & H1 & H2 & H3).
+    apply map_Excl_union_inv in H1 as (m1 & m2 & -> & -> & -> & Hdisj).
+    erewrite attach_owner_disj in Hdisj.
+    rewrite attach_owner_union map_Excl_union // auth_frag_op.
+    rewrite uPred.ownM_op.
+    iDestruct "H" as "[H1 H2]".
+    iSplitL "H1"; iExists _; iFrame; done.
+  - iDestruct "H" as "[H1 H2]".
+    iDestruct "H1" as (h1 H1) "H1".
+    iDestruct "H2" as (h2 H2) "H2".
+    iAssert ⌜ h1 ##ₘ h2 ⌝%I as %Hdisj.
+    {
+      iDestruct (uPred_ownM_disjoint with "H1 H2") as "H".
+      rewrite attach_owner_disj //.
+    }
+    iExists (h1 ∪ h2).
+    iSplitL "".
+    + iPureIntro. exists (map_Excl h1),(map_Excl h2).
+      repeat split; try done.
+      apply map_Excl_union. done.
+    + eapply attach_owner_disj in Hdisj.
+      rewrite attach_owner_union map_Excl_union // auth_frag_op uPred.ownM_op.
+      iFrame.
+Qed.
+
+Lemma owned_exists {A} (P : A -> oProp) o :
+  (∃ x, owned o (P x)) ⊣⊢ owned o (∃ x, P x).
+Proof.
+  unfold owned.
+  setoid_rewrite uPred_exists_holds.
+  iSplit; iIntros "H".
+  - iDestruct "H" as (x h H) "H".
+    iExists _. iFrame. iPureIntro. eauto.
+  - iDestruct "H" as (h [x H]) "H".
+    iExists _,_. iFrame. done.
+Qed.
+
+
+
+
+
+
+
+
+
+
+
+
+
+
+
+
+(*
+  =================================
+  TREES, OWN_AUTH, OWNI, OWNΔ, ETC.
+  =================================
+*)
+
+Definition G : Type. Admitted.
+Definition acyclic : G -> Prop. Admitted.
+Definition mk_graph : gmap endpoint owner -> G. Admitted.
+
+Section graph_lemmas.
+  Lemma acyclic_mk_delete Π l :
+    acyclic (mk_graph Π) -> acyclic (mk_graph (delete l Π)).
+  Proof.
+  Admitted.
+End graph_lemmas.
+
+Definition owners_valid (Δ : heapTO) (Σ : heapT) : Prop :=
+  Σ = fst <$> Δ ∧ acyclic (mk_graph $ snd <$> Δ).
+
+Section owners_valid.
+  Lemma owners_valid_lookup Δ Σ l t o :
+    owners_valid Δ Σ -> Δ !! l = Some (t,o) -> Σ !! l = Some t.
+  Proof.
+    intros [-> H].
+    rewrite lookup_fmap. intros ->. done.
+  Qed.
+
+  Lemma owners_valid_lookup_None Δ Σ l :
+    owners_valid Δ Σ ->
+    Δ !! l = None <-> Σ !! l = None.
+  Proof.
+    intros [-> H].
+    rewrite lookup_fmap.
+    destruct (Δ !! l) eqn:E; simpl; done.
+  Qed.
+
+  Lemma owners_valid_mutate Δ Σ l t t' o :
+    Δ !! l = Some (t, o) ->
+    owners_valid Δ Σ ->
+    owners_valid (<[l:=(t', o)]> Δ) (<[l:=t']> Σ).
+  Proof.
+    intros Hl [-> H].
+    split.
+    - rewrite fmap_insert. simpl. done.
+    - rewrite fmap_insert. simpl.
+      assert (<[l:=o]>(snd <$> Δ) = snd <$> Δ) as ->; last done.
+      apply insert_id.
+      rewrite lookup_fmap Hl. done.
+  Qed.
+
+  Lemma owners_valid_delete Δ Σ l t o :
+    Δ !! l = Some (t, o) ->
+    owners_valid Δ Σ ->
+    owners_valid (delete l Δ) (delete l Σ).
+  Proof.
+    intros Hl [-> H].
+    split.
+    - rewrite fmap_delete. done.
+    - rewrite fmap_delete. apply acyclic_mk_delete. done.
+  Qed.
+End owners_valid.
+
+Definition ownΔ (Δ : heapTO) : iProp := uPred_ownM (● (map_Excl Δ)).
+
+Definition own_auth (h : heapT) : iProp :=
+  ∃ Δ, ⌜⌜ owners_valid Δ h ⌝⌝ ∗ ownΔ Δ.
+
+Definition ownI (l : endpoint) (t : chan_type) (o : owner) : iProp :=
+  uPred_ownM (◯ {[ l := Excl (t,o) ]}).
+
+Definition ownO (l : endpoint) (t : chan_type) : oProp :=
+  uPred_ownM {[ l := Excl t ]}.
+
+Arguments uPred_holds {_} !_/.
+
+Lemma fmap_singleton_inv `{Countable K} {V1 V2} (f : V1 -> V2) (x : gmap K V1) (k : K) (v : V2) :
+  f <$> x = {[ k := v ]} -> ∃ v' : V1, x = {[ k := v' ]}.
+Proof.
+  intros HH.
+  rewrite ->map_eq_iff in HH.
+  pose proof (HH k) as H'.
+  rewrite lookup_fmap in H'.
+  rewrite lookup_singleton in H'.
+  destruct (x !! k) eqn:E; simpl in *; simplify_eq.
+  exists v0.
+  rewrite map_eq_iff.
+  intros. specialize (HH i).
+  rewrite lookup_fmap in HH.
+  destruct (decide (i = k)).
+  - subst. rewrite lookup_singleton in HH. rewrite lookup_singleton.
+    destruct (x !! k); simplify_eq. done.
+  - rewrite lookup_singleton_ne in HH; eauto.
+    rewrite lookup_singleton_ne; eauto.
+    destruct (x !! i); simplify_eq. done.
+Qed.
+
+Lemma singleton_eq_iff `{Countable K} {V} (k1 k2 : K) (v1 v2 : V) :
+  ({[ k1 := v1 ]} : gmap K V) = {[ k2 := v2 ]} <-> k1 = k2 ∧ v1 = v2.
+Proof.
+  split; last naive_solver.
+  intros HH.
+  rewrite ->map_eq_iff in HH.
+  specialize (HH k1).
+  rewrite lookup_singleton in HH.
+  destruct (decide (k1 = k2)); subst.
+  - rewrite lookup_singleton in HH. simplify_eq; done.
+  - rewrite lookup_singleton_ne in HH. simplify_eq. done.
+Qed.
+
+Lemma owned_own l t o :
+  ownI l t o ⊣⊢ owned o (ownO l t).
+Proof.
+  rewrite /ownI /owned /ownO.
+  iSplit.
+  - iIntros "H". iExists {[ l := t]}.
+    rewrite /attach_owner /map_Excl !map_fmap_singleton . iFrame.
+    iPureIntro. uPred.unseal. done.
+  - iIntros "H". iDestruct "H" as (h H) "H".
+    revert H. uPred.unseal. intros H.
+    rewrite -> leibniz_equiv_iff in H.
+    symmetry in H.
+    destruct (fmap_singleton_inv _ _ _ _ H) as [v' H'].
+    subst.
+    rewrite /map_Excl in H.
+    rewrite map_fmap_singleton in H.
+    apply singleton_eq_iff in H as []. simplify_eq.
+    rewrite /attach_owner /map_Excl !map_fmap_singleton //.
+Qed.
+
+Lemma ownI_lookup Δ l t o :
+  ownΔ Δ -∗ ownI l t o -∗ ⌜Δ !! l = Some (t, o)⌝.
+Proof.
+  iIntros "H1 H2".
+  iDestruct (uPred.ownM_op with "[H2 H1]") as "H"; first iFrame.
+  iDestruct (uPred.ownM_valid with "H") as "%".
+  iPureIntro.
+  apply auth_both_valid_discrete in H as [].
+  pose proof @singleton_included_exclusive_l.
+  specialize (H1 endpoint _ _ _ (Excl <$> Δ) l (Excl (t, o)) _ H0).
+  rewrite ->H1 in H.
+  rewrite lookup_fmap in H.
+  destruct (Δ !! l) eqn:E; simpl in *; simplify_eq. done.
+Qed.
+
+Lemma own_lookup Σ l t o :
+  own_auth Σ ∗ ownI l t o -∗ ⌜ Σ !! l = Some t ⌝.
+Proof.
+  iIntros "[H1 H2]".
+  iDestruct "H1" as (Δ HΔ) "H1".
+  iDestruct (ownI_lookup with "H1 H2") as %H.
+  iPureIntro.
+  eapply owners_valid_lookup; done.
+Qed.
+
+Lemma auth_update (a b a' b' : heapTO_UR) :
+  (a,b) ~l~> (a',b') → auth_global_update (● a ⋅ ◯ b) (● a' ⋅ ◯ b').
+Proof.
+  assert (Cancelable a) as Hcancel. { apply _. }
+  intros Hl.
+  rewrite ->local_update_unital in Hl.
+  rewrite /auth_global_update.
+  intros [[[q z1]|] z2] [H1 H2].
+  - rewrite view.view_valid_eq /= in H1.
+    destruct H1 as [H _].
+    apply Qp_not_add_le_l in H as [].
+  - rewrite view.view_valid_eq /= in H1.
+    destruct H1 as [_ H1].
+    specialize (H1 0). simpl in *.
+    destruct H1 as (x & ?%(inj _) & [z3 ?] & ?). simpl in *.
+    apply (inj Some) in H2 as [_ ?%(inj to_agree)]; simpl in *.
+    ofe_subst x.
+    assert (z3 ≡ ε).
+    {
+      eapply discrete; first apply _.
+      eapply Hcancel; first done.
+      rewrite {2}H0 right_id. done.
+    }
+    setoid_subst.
+    clear H0.
+    rewrite-> (right_id _ _) in H1.
+    destruct (Hl 0 z2); first done. { rewrite left_id. done. }
+    split.
+    + rewrite view.view_valid_eq /=.
+      split; first done.
+      exists a'.
+      split; first done.
+      split; last done.
+      rewrite left_id. apply discrete in H0; last apply _. setoid_subst. done.
+    + simpl in *.
+      do 2 constructor; simpl; first done.
+      f_equiv.
+      apply discrete in H0; last apply _.
+      by rewrite left_id.
+Qed.
+
+Lemma auth_update_alloc (a a' b' : heapTO_UR) :
+  (a,ε) ~l~> (a',b') → auth_global_update (● a) (● a' ⋅ ◯ b').
+Proof.
+  intros H.
+  assert (● a ≡ ● a ⋅ ε) as ->.
+  { rewrite right_id. done. }
+  by eapply auth_update.
+Qed.
+
+Definition change_owner (o : owner) (h : heapT) (Δ : heapTO) : heapTO. Admitted.
+
+(* Lemma owners_valid_chang_owner o o' :
+  connectedΔ Δ o o'
+  owners_valid Δ Σ ->
+  owners_valid (change_owner o h Δ) Σ *)
+
+Lemma own_move_tc Σ c t i P :
+  own_auth Σ ∗
+  ownI c t (Thread i) ∗
+  owned (Thread i) P
+  ==∗
+  own_auth Σ ∗
+  ownI c t (Thread i) ∗
+  owned (Chan c.1) P.
+Proof.
+  iIntros "(H1 & H2 & H3)".
+  rewrite /own_auth.
+  iDestruct "H1" as (Δ Hov) "H1".
+  iDestruct (ownI_lookup with "H1 H2") as %H.
+  rewrite /owned.
+  iDestruct "H3" as (h Hh) "H3".
+  iDestruct (uPred.ownM_op with "[H3 H1]") as "H"; first iFrame.
+  iMod (bupd_ownM_update with "H") as "H".
+  {
+    eapply (auth_update _ _
+        (map_Excl (change_owner (Chan c.1) h Δ))
+        (map_Excl (attach_owner (Chan c.1) h))).
+    rewrite /attach_owner.
+    admit.
+    (* eapply (auth_update _ _ (Excl <$> (<[ l := (t',o) ]> Δ)) {[l := Excl (t', o)]}). *)
+  }
+  iFrame.
+  rewrite uPred.ownM_op.
+  iDestruct "H" as "[H1 H3]".
+  iModIntro.
+  iSplitL "H1".
+  - iExists _. iFrame. iPureIntro.
+
+    admit.
+  - iExists _. iFrame. iPureIntro. done.
+Admitted.
+
+Lemma own_move_ct Σ c t i P :
+  own_auth Σ ∗
+  ownI c t (Thread i) ∗
+  owned (Chan c.1) P
+  ==∗
+  own_auth Σ ∗
+  ownI c t (Thread i) ∗
+  owned (Thread i) P.
+Proof. Admitted.
+
+Lemma own_alloc (i i' : nat) (l : endpoint) (Σ : heapT) (t t' : chan_type) :
+  i ≠ i' →
+  Σ !! l = None →
+  Σ !! other l = None →
+  own_auth Σ ==∗
+     own_auth (<[l:=t]> $ <[other l:=t']> Σ) ∗
+     ownI l t (Thread i) ∗ ownI (other l) t' (Thread i').
+Proof.
+  iIntros (Hi H1 H2) "H".
+  rewrite /own_auth.
+  iDestruct "H" as (Δ Hov) "H".
+  rewrite /ownΔ.
+  rewrite <-owners_valid_lookup_None in H1; last done.
+  rewrite <-owners_valid_lookup_None in H2; last done.
+  iMod (bupd_ownM_update with "H") as "H".
+  {
+    assert (● map_Excl Δ ≡ ● map_Excl Δ ⋅ ε) as ->.
+    { rewrite right_id. done. }
+    eapply auth_update.
+    assert (map_Excl Δ !! l = None).
+    { rewrite /map_Excl lookup_fmap H1. done. }
+    assert (map_Excl Δ !! other l = None).
+    { rewrite /map_Excl lookup_fmap H2. done. }
+    eapply transitivity.
+    - eapply (alloc_local_update _ _ l (Excl (t,Thread i))); try done.
+    - eapply (alloc_local_update _ _ (other l) (Excl (t',Thread i'))); try done.
+      rewrite /map_Excl lookup_insert_ne //.
+      destruct l. simpl. destruct b; done.
+  }
+  rewrite /ownI.
+  rewrite -!map_Excl_insert.
+  rewrite !map_Excl_insert_op //.
+  2: { rewrite lookup_insert_ne //. apply other_neq. }
+  rewrite insert_singleton_op.
+  2: { rewrite lookup_insert_ne //. apply other_neq. }
+  rewrite insert_empty.
+  rewrite auth_frag_op.
+  rewrite !uPred.ownM_op.
+  iDestruct "H" as "(H1 & H2 & H3)". iFrame.
+  rewrite -!map_Excl_insert_op //.
+  2: { rewrite lookup_insert_ne //. apply other_neq. }
+  iModIntro. iExists _. iFrame.
+  iPureIntro.
+  (* Need to track which threads are fresh in Δ:
+      own_auth Σ -> own_auth Σ k
+     where k is the current number of threads.
+     Then this lemma does own_auth Σ k -> own_auth Σ' (k + 1) *)
+  admit.
+Admitted.
+
+Lemma own_mutate Σ l t t' o :
+  own_auth Σ ∗ ownI l t o ==∗ own_auth (<[l:=t']> Σ) ∗ ownI l t' o.
+Proof.
+  iIntros "[H1 H2]".
+  iDestruct "H1" as (Δ Hov) "H1".
+  iDestruct (ownI_lookup with "H1 H2") as %Hl.
+  iDestruct (uPred.ownM_op with "[H2 H1]") as "H"; first iFrame.
+  iMod (bupd_ownM_update with "H") as "H".
+  { eapply (auth_update _ _ (Excl <$> (<[ l := (t',o) ]> Δ)) {[l := Excl (t', o)]}).
+    rewrite !fmap_insert.
+    assert ({[l := Excl (t', o)]} = <[ l:= Excl (t',o) ]> ({[l := Excl (t, o)]} : gmap _ _)).
+    { rewrite insert_singleton. done. }
+    rewrite H.
+    eapply insert_local_update.
+    - rewrite lookup_fmap. rewrite Hl. simpl. done.
+    - rewrite lookup_singleton. done.
+    - by apply exclusive_local_update.
+  }
+  iModIntro.
+  rewrite /ownI /own_auth. iFrame.
+  rewrite uPred.ownM_op.
+  iDestruct "H" as "[H1 H2]".
+  iFrame.
+  iExists _.
+  iFrame.
+  iPureIntro.
+  eapply owners_valid_mutate; eauto.
+Qed.
+
+Lemma own_dealloc Σ l t o :
+  own_auth Σ ∗ ownI l t o ==∗ own_auth (delete l Σ).
+Proof.
+  iIntros "[H1 H2]".
+  iDestruct "H1" as (Δ Hov) "H1".
+  iDestruct (ownI_lookup with "H1 H2") as %Hl.
+  iDestruct (uPred.ownM_op with "[H2 H1]") as "H"; first iFrame.
+  iMod (bupd_ownM_update with "H") as "H".
+  {
+    eapply (auth_update _ _ (Excl <$> (delete l Δ)) ∅).
+    rewrite fmap_delete.
+    eapply delete_singleton_local_update.
+    apply _.
+  }
+  iModIntro.
+  rewrite uPred_primitive.ownM_op.
+  iDestruct "H" as "[H1 H2]".
+  rewrite uPred.ownM_unit.
+  iExists _. iFrame.
+  iPureIntro.
+  eapply owners_valid_delete; done.
+Qed.
+
+
+(*
+Lemma strong_adequacy {A : ucmraT} (φ : A -> A -> Prop) :
+  (uPred_ownM (● ε) ⊢ |==> ∃ x y, uPred_ownM (● x ⋅ ◯ y) ∧ ⌜ φ x y ⌝) → ∃ x, φ x x.
+Proof.
+Admitted.
+
+Lemma P_to_own_frag {A : ucmraT} (x : A) (P : uPred A) :
+  uPred_ownM (● x) ∗ P ⊢ ∃ y, uPred_ownM (● x ⋅ ◯ y).
+Proof.
+Admitted.
+ *)
+
+(* Lemma allocate Σ l t o :
+  Σ !! l = None →
+  own_auth Σ ⊢ |==> own_auth (<[l:=(t,o)]> Σ) ∗ own l t o.
+Proof.
+  intros H.
+  rewrite own_ownM.
+  apply uPred.bupd_ownM_update.
+  apply auth_update_alloc; first apply _.
+  rewrite fmap_insert.
+Admitted. *)
+  (* Check alloc_singleton_local_update.
+  apply alloc_singleton_local_update; last done.
+  by rewrite lookup_fmap H.
+Qed. *)
+
+(* Lemma auth_update_dealloc {A:ucmraT} (a b a' : A) :
+  Cancelable a →
+  (a,b) ~l~> (a',ε) → uPred_primitive.auth_global_update (● a ⋅ ◯ b) (● a').
+Proof.
+  intros Hcancel Hl.
+  eapply uPred_primitive.auth_global_update_proper, auth_update, Hl; auto.
+  rewrite (_ : (◯ ε) = ε); last done.
+  by rewrite right_id.
+Qed. *)
+
+(* Lemma deallocate Σ l t o :
+  own_auth Σ ∗ own l t o ⊢ |==> own_auth (delete l Σ).
+Proof.
+  iIntros "H".
+  iDestruct (own_lookup with "H") as "%".
+  iStopProof.
+  rewrite own_ownM.
+  apply uPred.bupd_ownM_update.
+  apply auth_update_dealloc; first apply _.
+  rewrite fmap_delete.
+Admitted.
+  apply delete_singleton_local_update_cancelable; first apply _.
+  rewrite lookup_fmap. rewrite H. done.
+Qed. *)
+
+(* Lemma update Σ l t t' :
+  own_auth Σ ∗ own l t ⊢
+  |==> own_auth (<[l:=t']> Σ) ∗ own l t'.
+Proof.
+  iIntros "[H1 H2]".
+  iApply bupd_trans.
+  replace (<[l:=t']> Σ) with (<[l := t']> (delete l Σ))
+    by apply fin_maps.insert_delete.
+  iApply allocate. { apply lookup_delete. }
+  iApply deallocate. iFrame.
+Qed. *)
+
+
+(* Lemma adequacy φ :
+  (own_auth ∅ ⊢ |==> ∃ Σ2, own_auth Σ2 ∧ ⌜ φ Σ2 ⌝) → φ ∅.
+Proof.
+  unfold own_auth.
+  intros HH.
+  destruct (uPred.ownM_soundness (M:= heapTUR) (● ε)
+    (λ x, ∃ y, x ≡ ● (Excl <$> y) ∧ φ y)) as [x [H1 [y [H2 H3]]]].
+  - apply _.
+  - split; last done.
+    by apply auth_auth_validN.
+  - iIntros "H".
+    iMod (HH with "[H]") as (Σ) "[H %]".
+    + by rewrite fmap_empty.
+    + iExists (● (Excl <$> Σ)). iFrame.
+      iModIntro. iSplit; first done.
+      iPureIntro.
+      by exists Σ.
+  - unfold uPred_primitive.auth_global_updateN in H1.
+    destruct (H1 ε) as [R1 R2].
+    { split. rewrite right_id. by apply auth_auth_validN.
+      simpl. by rewrite !right_id. }
+    simpl in *.
+    rewrite right_id in R2.
+    rewrite-> H2 in R2.
+    simpl in *.
+    apply (inj Some) in R2 as [_ R2]. simpl in *.
+    apply (inj to_agree) in R2.
+    rewrite-> (left_id _ _) in R2.
+    apply (discrete _) in R2.
+    apply leibniz_equiv_iff in R2.
+    by apply (fmap_empty_inv Excl) in R2 as ->.
+Qed. *)
+
+(* Lemma auth_global_valid_auth {A : ucmraT} n :
+  auth_global_valid n (● (ε : A)).
+Proof.
+  split; last done.
+  apply auth_auth_validN. apply ucmra_unit_validN.
+Qed.
+
+Lemma simple_adequacy φ :
+  (own_auth ∅ ⊢ |==> ⌜ φ ⌝) → φ.
+Proof. Admitted. *)
+  (* unfold own_auth.
+  apply uPred.ownM_simple_soundness.
+  rewrite fmap_empty.
+  apply: auth_global_valid_auth.
+Qed. *)
