theories/typescourse/tait5.v
@@ -1,0 +1,19 @@
+Inductive expr :=
+  | Pred : expr -> expr
+  | Inl : expr -> expr
+  | Inr : expr -> expr
+  | Unit : expr.
+  (* and more... *)
+
+Inductive steps : expr -> expr -> Prop := . (* step relation... *)
+
+CoInductive conat_eq : expr -> expr -> Prop :=
+  | zero_eq e1 e2 :
+    steps (Pred e1) (Inl Unit) ->
+    steps (Pred e2) (Inl Unit) ->
+    conat_eq e1 e2
+  | succ_eq e1 e2 e1' e2' :
+    steps (Pred e1) (Inr e1') ->
+    steps (Pred e2) (Inr e2') ->
+    conat_eq e1' e2' ->
+    conat_eq e1 e2.
